Attempt to prove some useful lemmas about speculative VLSMs, but failed so far.

theories/VLSM/Core/Speculation.v
@@ -92,4 +92,151 @@ Definition speculative_vlsm : VLSM message :=
   vmachine := speculative_vlsm_machine;
 |}.
 
+Lemma valid_state_prop_Actual :
+  forall (s : vstate X),
+    valid_state_prop X s -> valid_state_prop speculative_vlsm (Actual s).
+Proof.
+  intros s [om Hvsmp]; red.
+  induction Hvsmp.
+  - by exists None; constructor; cbn.
+  - destruct IHHvsmp1 as [om1 Hom1], IHHvsmp2 as [om2 Hom2].
+    exists om1.
+    Print valid_state_message_prop.
+    Check valid_generated_state_message _ _ _ Hom1 _ _ Hom2.
+Admitted.
+
+Lemma speculative_option_valid_message_prop_None :
+  option_valid_message_prop speculative_vlsm None.
+Proof.
+Admitted.
+
+Lemma input_valid_transition_Speculate :
+  forall (s : vstate X) (plan : list (vplan_item X)),
+    valid_state_prop X s -> plan <> [] ->
+      input_valid_transition speculative_vlsm
+        (Speculate plan) (Actual s, None) (Speculative s s plan [], None).
+Proof.
+  intros s plan Hvsp Hplan.
+  constructor; cbn; [| done].
+  split_and!; [.. | done].
+  - by apply valid_state_prop_Actual.
+  - by apply speculative_option_valid_message_prop_None.
+Qed.
+
+Lemma input_valid_transition_Execute :
+  forall (lbl : label) (start current current' : vstate X) (msg om : option message)
+    (plan : list (vplan_item X)) (outputs : list (option message)),
+    input_valid_transition X lbl (current, msg) (current', om) ->
+      input_valid_transition speculative_vlsm Execute
+        (Speculative start current (Build_plan_item lbl msg :: plan) outputs, None)
+        (Speculative start current' plan (outputs ++ [om]), None).
+Proof.
+  intros.
+Admitted.
+
+Lemma input_valid_transition_Commit_cons :
+  forall (start current : vstate X) (om : option message) (outputs : list (option message)),
+    valid_state_prop speculative_vlsm (Speculative start current [] (om :: outputs)) ->
+      input_valid_transition speculative_vlsm Commit
+        (Speculative start current [] (om :: outputs), None)
+        (Speculative start current [] outputs, om).
+Proof.
+  constructor; cbn; [| done].
+  split_and!; [done | | done].
+  by apply speculative_option_valid_message_prop_None.
+Qed.
+
+Lemma input_valid_transition_Commit_nil :
+  forall (start current : vstate X),
+    valid_state_prop speculative_vlsm (Speculative start current [] []) ->
+      input_valid_transition speculative_vlsm Commit
+        (Speculative start current [] [], None) (Actual current, None).
+Proof.
+  constructor; cbn; [| done].
+  split_and!; [done | | done].
+  by apply speculative_option_valid_message_prop_None.
+Qed.
+
+Print transition_item.
+
+Fixpoint speculative_lift_trace
+  (start : vstate X) (tr : list (@transition_item _ (vtype X)))
+  : list (@transition_item _ speculative_vlsm_type) :=
+match tr with
+| [] => []
+| Build_transition_item lbl iom current oom :: tr' =>
+    let plan := [Build_plan_item lbl iom]
+    in
+    let spec := @Build_transition_item _ speculative_vlsm_type
+          (Speculate plan) None (Speculative start start plan []) None
+    in
+    let exec := @Build_transition_item _ speculative_vlsm_type
+          Execute None (Speculative start current [] [oom]) None
+    in
+    let out := @Build_transition_item _ speculative_vlsm_type
+          Commit None (Speculative start current [] []) oom
+    in
+    let commit := @Build_transition_item _ speculative_vlsm_type
+          Commit None (Actual current) None
+    in
+      spec :: exec :: out :: commit :: speculative_lift_trace current tr'
+end.
+
+Lemma in_futures_speculative :
+  forall (s1 s2 : vstate X),
+    in_futures X s1 s2 -> in_futures speculative_vlsm (Actual s1) (Actual s2).
+Proof.
+  intros s1 s2 [tr Htr].
+  unfold in_futures.
+  induction Htr.
+  + exists []; constructor.
+    by apply valid_state_prop_Actual.
+  + destruct IHHtr as [tr IH].
+    pose (plan := [Build_plan_item l iom]).
+    pose (spec := @Build_transition_item _ speculative_vlsm_type
+      (Speculate plan) None (Speculative s' s' plan []) None).
+    pose (exec := @Build_transition_item _ speculative_vlsm_type
+      Execute None (Speculative s' s [] [oom]) None).
+    pose (out := @Build_transition_item _ speculative_vlsm_type
+      Commit None (Speculative s' s [] []) oom).
+    pose (commit := @Build_transition_item _ speculative_vlsm_type
+      Commit None (Actual s) None).
+    exists (spec :: exec :: out :: commit :: tr).
+    inversion Ht as [[Ht1 [Ht2 Ht3]] Ht4].
+    constructor; [| by eapply input_valid_transition_Speculate].
+    constructor; cycle 1.
+    * unfold plan; change [oom] with ([] ++ [oom]).
+      by eapply input_valid_transition_Execute.
+    * constructor; cycle 1.
+      -- apply input_valid_transition_Commit_cons. admit.
+      -- constructor; [done |].
+         red; cbn.
+         split_and!; [admit | | done..].
+         by apply speculative_option_valid_message_prop_None.
+Admitted.
+
+Lemma in_futures_speculative' :
+  forall (s1 s2 : vstate X),
+    in_futures X s1 s2 -> in_futures speculative_vlsm (Actual s1) (Actual s2).
+Proof.
+  intros s1 s2 [tr Htr].
+  unfold in_futures.
+  exists (speculative_lift_trace s1 tr).
+  induction Htr.
+  - cbn; constructor.
+    by apply valid_state_prop_Actual.
+  - inversion Ht as [[Ht1 [Ht2 Ht3]] Ht4].
+    simpl.
+    constructor; [| by eapply input_valid_transition_Speculate].
+    constructor; cycle 1.
+    + change [oom] with ([] ++ [oom]).
+      by eapply input_valid_transition_Execute.
+    + constructor; cycle 1.
+      * apply input_valid_transition_Commit_cons. admit.
+      * constructor; cbn; [done |].
+        red; cbn.
+        split_and!; [admit | | done..].
+        by apply speculative_option_valid_message_prop_None.
+Admitted.
+
 End sec_speculative.
